extract_ocaml.v
@@ -12,35 +12,5 @@ Extract Inductive list => "list" [ "[]" "(::)" ].
 Extract Inductive prod => "( * )" [ "( , )" ].
 Extract Inductive sumbool => "bool" ["true" "false"].
 
-(*
-Extract Inductive nat => int [ "0" "Stdlib.Int.succ" ]
- "(fun fO fS n -> if n=0 then fO () else fS (n-1))".
-
-
-Extract Constant plus => "(+)".
-Extract Constant pred => "fun n -> Stdlib.max 0 (n-1)".
-Extract Constant minus => "fun n m -> Stdlib.max 0 (n-m)".
-Extract Constant mult => "( * )".
-Extract Inlined Constant max => "Stdlib.max".
-Extract Inlined Constant min => "Stdlib.min".
-Extract Inlined Constant Nat.eqb => "(=)".
-Extract Inlined Constant EqNat.eq_nat_decide => "(=)".
-
-Extract Inlined Constant Peano_dec.eq_nat_dec => "(=)".
-
-Extract Constant Nat.compare =>
- "fun n m -> if n=m then Eq else if n<m then Lt else Gt".
-Extract Inlined Constant Compare_dec.leb => "(<=)".
-Extract Inlined Constant Compare_dec.le_lt_dec => "(<=)".
-Extract Inlined Constant Compare_dec.lt_dec => "(<)".
-Extract Constant Compare_dec.lt_eq_lt_dec =>
- "fun n m -> if n>m then None else Some (n<m)".
-
-*)
-
-(** Program Extractions **)
-(*  Examples from example.v are extracted and directly tested.
-    After running the next line, use "make run" in order to compile and
-    run the test_examples.ml file. *)
 Extraction Parser.
 Extraction "ocaml_interface/checker.ml" Parser. 
